intermediate/Veritas.Intermediate.Store.fsti
@@ -283,7 +283,7 @@ val mevict_from_store
 val bevict_from_store
   (#vcfg: verifier_config)
   (st:vstore vcfg)
-  (s:inuse_slot_id st{points_to_none st s Left /\ points_to_none st s Right})
+  (s:inuse_slot_id st{points_to_none st s Left /\ points_to_none st s Right /\ add_method_of st s = Spec.BAdd})
   : Tot (st':vstore vcfg {// st and st' are identical except at slot s
                           identical_except st st' s /\
 
@@ -461,7 +461,7 @@ val lemma_not_contains_after_mevict
 val lemma_not_contains_after_bevict
   (#vcfg: verifier_config)
   (st:vstore vcfg)
-  (s:inuse_slot_id st{points_to_none st s Left /\ points_to_none st s Right})
+  (s:inuse_slot_id st{points_to_none st s Left /\ points_to_none st s Right /\ add_method_of st s = Spec.BAdd})
   : Lemma (ensures (let st' = bevict_from_store st s in
                     let k = stored_key st s in
                     is_map st' /\
